Isabelle: Sketch the local confluence proof for the root overlap of SubstRec

isabelle/LocalConfluence.thy
@@ -72,6 +72,222 @@ lemma Unify_Seql_Unify_Seqr: "rule_Unify_Seql\<inverse>\<inverse> OO rule_Unify_
 lemma Unify_Seqr_Unify_Seqr: "rule_Unify_Seqr\<inverse>\<inverse> OO rule_Unify_Seqr \<le> J"
   by(auto intro!: joinI elim!: rule_Unify_Seqr.cases)
 
+(* Subst-rec is not yet part of Rs, but here is its own little diagram *)
+
+consts subVC :: "vc \<Rightarrow> vc \<Rightarrow> exp \<Rightarrow> vc"
+
+lemma subVC_eq:
+  assumes  "vc1 \<noteq> vc2"
+  assumes  "appVC vc1 e1 = appVC vc2 e2"
+  shows    "subVC vc1 vc2 e2 = vc1"
+  sorry
+
+lemma subVC_swap:
+  assumes  "vc1 \<noteq> vc2"
+  shows    "appVC (subVC vc1 vc2 e2) e1 = appVC (subVC vc2 vc1 e1) e2"
+  sorry
+
+lemma liftVC_subVC:
+  "liftVC n k (subVC vc1 vc2 e) = subVC (liftVC n k vc1) (liftVC n k vc2) (liftE n (Suc k) e)"
+  sorry
+
+lemma substVC_subVC:
+  "substVC n v (subVC vc1 vc2 e) = subVC (substVC n v vc1) (substVC n v vc2) (substE (Suc n) (liftV 1 0 v) e)"
+  sorry
+
+lemma liftV_appVC[simp]: "liftV n k (appVC vc e) = appVC (liftVC n k vc) (liftE n (Suc k) e)"
+  sorry
+
+lemma substV_appVC[simp]: "substV n v (appVC vc e) = appVC (substVC n v vc) (substE (Suc n) (liftV 1 0 v) e)"
+  sorry
+
+lemma liftVC_substVC:
+  "liftVC k j (substVC n v vc) =
+    (if n < j then substVC n (liftV k j v) (liftVC k j vc)
+    else substVC (n+k) (liftV k j v) (liftVC k j vc))"
+  sorry
+
+lemma substVC_dead:
+  "\<not> occursVC n vc \<Longrightarrow> substVC n v vc = vc"
+  sorry
+
+
+lemma liftVC_liftVC[simp]:
+  "l \<le> k2 \<Longrightarrow> k2 \<le> j+l \<Longrightarrow> liftVC k k2 (liftVC j l vc) = liftVC (k+j) l vc"
+  sorry
+
+lemma liftVC_liftVC_sort[simp]:
+  "k2 < l \<Longrightarrow> liftVC k k2 (liftVC j l vc) = liftVC j (l+k) (liftVC k k2 vc)"
+  sorry
+
+lemma substVC_again[simp]:
+  "\<not> occursV n v2 \<Longrightarrow> substVC n v1 (substVC n v2 vc) = substVC n v2 vc"
+  sorry
+
+
+lemma substVC_substVC:
+  "\<not> occursV n2 v1 \<Longrightarrow>
+  substVC n1 v1 (substVC n2 v2 vc) = substVC n2 (substV n1 v1 v2) (substVC n1 v1 vc)"
+  sorry
+
+lemma liftE_substE:
+  "liftE k j (substE n v e) =
+    (if n < j then substE n (liftV k j v) (liftE k j e)
+    else substE (n+k) (liftV k j v) (liftE k j e))"
+  sorry
+
+lemma substE_dead:
+  "\<not> occursE n e \<Longrightarrow> substE n v e = e"
+  sorry
+
+lemma liftE_liftE[simp]:
+  "l \<le> k2 \<Longrightarrow> k2 \<le> j+l \<Longrightarrow> liftE k k2 (liftE j l e) = liftE (k+j) l e"
+  sorry
+
+lemma liftE_liftE_sort[simp]:
+  "k2 < l \<Longrightarrow> liftE k k2 (liftE j l e) = liftE j (l+k) (liftE k k2 e)"
+  sorry
+
+
+lemma substE_again[simp]:
+  "\<not> occursV n v2 \<Longrightarrow> substE n v1 (substE n v2 e) = substE n v2 e"
+  sorry
+
+
+lemma substE_substE:
+  "\<not> occursV n2 v1 \<Longrightarrow>
+  substE n1 v1 (substE n2 v2 e) = substE n2 (substV n1 v1 v2) (substE n1 v1 e)"
+  sorry
+
+lemma arg_cong3: "\<lbrakk>a = b; c = d; e = g\<rbrakk> \<Longrightarrow> f a c e = f b d g"
+  by (iprover intro: refl elim: subst)
+
+
+lemma Subst_Rec_Subst_Rec: "rule_SubstRec\<inverse>\<inverse> OO rule_SubstRec \<le> (cc rule_SubstRec)\<^sup>*\<^sup>* OO (cc rule_SubstRec)\<^sup>*\<^sup>*\<inverse>\<inverse>"
+proof(rule joinI; elim rule_SubstRec.cases; clarify; goal_cases)
+  case (1 _ _ _ _ e1 _ vc1 _ n e2 _ vc2 _)
+
+  let "(((cc rule_SubstRec)\<^sup>*\<^sup>* OO (cc rule_SubstRec)\<^sup>*\<^sup>*\<inverse>\<inverse>) ?left ?right)" = "?case"
+  let ?letUnderLam = "\<lambda> n vc rhs e. Uni (Val (Var n)) (Val (appVC vc (Def (Seq (Uni (Val (Var 0)) (Val rhs)) e))))"
+  let "Uni (Val (Var n)) (Val (appVC vc1 (Def (Seq (Uni (Val (Var 0)) (Val ?rhs1)) ?e1'))))" = "?left"
+  let "Uni (Val (Var n)) (Val (appVC vc2 (Def (Seq (Uni (Val (Var 0)) (Val ?rhs2)) ?e2'))))" = "?right"
+
+  have "?letUnderLam n vc1 ?rhs1 ?e1' = ?left".. (* sanity check *)
+
+  show ?case
+  proof(cases "vc1 = vc2")
+    case True
+    with `appVC _ _ = _`
+    have "e1 = e2" by auto
+    hence "?letUnderLam n vc1 ?rhs1 ?e1' = ?letUnderLam n vc2 ?rhs2 ?e2'" using True by simp
+    then show ?thesis by auto
+  next
+    case False
+
+    have vc1_sub: "\<And> e1. appVC vc1 e1 = appVC (subVC vc2 vc1 e1) e2"
+      by (metis "1"(3) False subVC_eq subVC_swap)
+
+    have vc2_sub: "\<And> e2. appVC vc2 e2 = appVC (subVC vc1 vc2 e2) e1"
+      by (metis "1"(3) False subVC_eq subVC_swap)
+
+    have helper: "\<And> P x y. x = y \<Longrightarrow> P\<^sup>*\<^sup>* x y" by simp
+
+    have inj: "substVC (Suc (Suc n)) (Var 0) (liftVC 2 0 vc1) \<noteq>
+              substVC (Suc (Suc n)) (Var 0) (liftVC 2 0 vc2)" sorry
+
+    show ?thesis
+      apply (rule relcomppI)
+       apply (rule rtranclp_trans[OF r_into_rtranclp r_into_rtranclp])
+        apply (simp only: liftV_appVC substV_appVC)
+        apply (subst vc1_sub)
+        apply (rule cc_rootI)
+        apply (rule rule_SubstRec[OF _ refl refl])
+        apply (rule `occursE (n+1) e2`)
+      apply (subst subVC_swap[OF False[symmetric]])
+      apply (rule congruentE[OF congruent_cc, of _ _ _  "[CUnir e]" for e, simplified appEC_def, simplified])
+      apply (rule congruentE[OF congruent_cc, of _ _ _  "[CVal vc]" for vc, simplified appEC_def, simplified])
+      apply (rule congruentE[OF congruent_cc, of _ _ _  "[CDef]", simplified appEC_def, simplified])
+       apply (rule congruentE[OF congruent_cc, of _ _ _  "[CSeql e]" for e, simplified appEC_def, simplified])
+       apply (rule cc_rootI)
+       apply (simp only: liftV_appVC[symmetric] substV_appVC[symmetric]) 
+       apply (subst vc1_sub)
+       apply (simp only: liftV_appVC substV_appVC) 
+       apply (rule rule_SubstRec[OF _ refl refl])
+      using  `occursE (n+1) e2` apply (simp add: occursE_liftE)
+      apply (rule conversepI)
+       apply (rule rtranclp_trans[OF r_into_rtranclp rtranclp_trans[OF r_into_rtranclp helper]])
+        apply (simp only: liftV_appVC substV_appVC)
+        apply (subst vc2_sub)
+        apply (rule cc_rootI)
+        apply (rule rule_SubstRec[OF _ refl refl])
+       apply (rule `occursE (n+1) e1`)
+      apply (subst subVC_swap[OF False])
+      apply (rule congruentE[OF congruent_cc, of _ _ _  "[CUnir e]" for e, simplified appEC_def, simplified])
+      apply (rule congruentE[OF congruent_cc, of _ _ _  "[CVal vc]" for vc, simplified appEC_def, simplified])
+      apply (rule congruentE[OF congruent_cc, of _ _ _  "[CDef]", simplified appEC_def, simplified])
+       apply (rule congruentE[OF congruent_cc, of _ _ _  "[CSeql e]" for e, simplified appEC_def, simplified])
+       apply (rule cc_rootI)
+       apply (simp only: liftV_appVC[symmetric] substV_appVC[symmetric]) 
+       apply (subst vc2_sub)
+       apply (simp only: liftV_appVC substV_appVC) 
+       apply (rule rule_SubstRec[OF _ refl refl])
+      using  `occursE (n+1) e1` apply (simp add: occursE_liftE)
+      (* Now we have to show that the result is the same *)
+      apply (simp add: subVC_swap[OF False])
+      apply (rule arg_cong2[where f = "\<lambda> e1 e2. appVC (subVC vc2 vc1 e1) e2" for vc1 vc2])
+      apply (rule arg_cong2[where f = VLet])
+        apply (rule arg_cong2[where f = appVC])
+         apply simp
+      apply (rule arg_cong2[where f = VLet])
+         apply (rule arg_cong2[where f = appVC])
+          apply (subst subVC_eq[OF False[symmetric] "1"(3)[symmetric]])
+          apply (simp add: liftVC_substVC)
+          apply (subst substVC_substVC)
+           apply simp
+          apply (simp add: substVC_dead)
+          apply (simp add: liftE_substE)
+          apply (subst substE_substE)
+           apply simp
+         apply (simp add: substE_dead occursE_liftE)
+          apply (simp add: liftE_substE)
+          apply (subst substE_substE)
+           apply simp
+        apply (simp add: substE_dead occursE_liftE)
+       apply simp
+      apply (rule arg_cong2[where f = VLet])
+       apply (simp add: liftVC_subVC substVC_subVC subVC_swap[OF inj])
+      apply (rule arg_cong2[where f = "\<lambda> e1 e2. appVC (subVC vc2 vc1 e1) e2" for vc1 vc2])
+      apply (rule arg_cong2[where f = VLet])
+         apply (rule arg_cong2[where f = appVC])
+          apply (subst (2) subVC_eq[OF False "1"(3), symmetric])
+          apply (simp add: liftVC_subVC substVC_subVC)
+          apply (rule arg_cong3[where f = subVC])
+            apply (simp add: liftVC_substVC)
+            apply (subst substVC_substVC)
+             apply simp
+            apply (simp add: substVC_dead)
+           apply (simp add: liftVC_substVC)
+           apply (subst substVC_substVC)
+            apply simp
+           apply (simp add: substVC_dead)
+          apply (simp add: liftE_substE)
+          apply (subst substE_substE)
+           apply simp
+         apply (simp add: substE_dead occursE_liftE)
+          apply (simp add: liftE_substE)
+          apply (subst substE_substE)
+           apply simp
+         apply (simp add: substE_dead occursE_liftE)
+          apply (simp add: liftE_substE)
+          apply (subst substE_substE)
+           apply simp
+         apply (simp add: substE_dead occursE_liftE)
+       apply simp
+      apply simp
+      done
+  qed
+qed
+
 
 lemma mirror_elementary:
   assumes "R1\<inverse>\<inverse> OO R2 \<le> J"
